theories/Runtime/SmallStepRuntimeSubstShape.v
@@ -113,10 +113,10 @@ Lemma WTStateRuntimeSubstShape_not_stuck :
 Proof.
   intros state tout HState HEvalReady.
   destruct HState.
-  - right.
+  - right. left.
     destruct (HEvalReady heap env rho e k eq_refl) as [HSeq HResolved].
     eapply typed_eval_sequential_head_progress_unindexed; eauto.
-  - right.
+  - right. left.
     eapply typed_return_runtime_shape_progress; eauto.
   - left. constructor.
 Qed.
@@ -285,4 +285,3 @@ Proof.
   rewrite subst_rho_tyref.
   now rewrite subst_rho_rgn_const.
 Qed.
-
